qcp-binary-democases/QCP_examples/hashtbl_def.h
@@ -46,6 +46,7 @@ struct hashtbl {
                (fst: {A} {B} -> A * B -> A)
                (snd: {A} {B} -> A * B -> B)
                (pair: {A} {B} -> A -> B -> A * B)
+               (In: {A} -> A -> list A -> Prop)
  */
 
 /*@ Import Coq Require Import hashtbl_lib */
