HashTable/hashtbl_proof_manual.v
@@ -1,0 +1,836 @@
+(* Require Import Coq.ZArith.ZArith.
+Require Import Coq.Bool.Bool.
+Require Import Coq.Strings.String.
+Require Import Coq.Lists.List.
+Require Import Coq.Classes.RelationClasses.
+Require Import Coq.Classes.Morphisms.
+Require Import Coq.micromega.Psatz.
+Require Import Coq.Sorting.Permutation.
+From AUXLib Require Import int_auto Axioms Feq Idents List_lemma VMap.
+Require Import SetsClass.SetsClass. Import SetsNotation.
+From SimpleC.SL Require Import Mem SeparationLogic MapLib CommonAssertion.
+Require Import Logic.SeparationLogic.ProofTheory.SeparationLogic.
+Require Import hashtbl_goal.
+Require Import Logic.LogicGenerator.demo932.Interface.
+Local Open Scope Z_scope.
+Local Open Scope sets.
+Local Open Scope string.
+Local Open Scope list.
+Import naive_C_Rules.
+Require Import hashtbl_lib.
+Local Open Scope sac.
+
+Module BV.
+  Definition insert_map {A} (m: Z -> option A) (k: Z) (v: A) : Z -> option A :=
+    fun x => if Z.eq_dec x k then Some v else m x.
+
+  Lemma insert_map_same {A} : forall (m: Z -> option A) k v,
+    insert_map m k v k = Some v.
+  Proof.
+    intros. unfold insert_map. destruct (Z.eq_dec k k); congruence.
+  Qed.
+
+  Lemma insert_map_diff {A} : forall (m: Z -> option A) k1 k2 v,
+    k1 <> k2 -> insert_map m k1 v k2 = m k2.
+  Proof.
+    intros. unfold insert_map. destruct (Z.eq_dec k2 k1); congruence.
+  Qed.
+
+  Lemma insert_map_iff {A} : forall (m: Z -> option A) k v p,
+    insert_map m k v p <> None <-> (p = k \/ m p <> None).
+  Proof.
+    intros. unfold insert_map. destruct (Z.eq_dec p k).
+    - subst. split; intros.
+      + left; auto.
+      + congruence.
+    - split; intros.
+      + right. auto.
+      + destruct H; try congruence.
+  Qed.
+End BV.
+
+
+
+
+
+(* ---------------------------------------------------------------------- *)
+(* Helper lemmas about lists                                               *)
+(* ---------------------------------------------------------------------- *)
+
+Lemma firstn_replace_nth_nat {A} (n: nat) (v: A) (l: list A) :
+  firstn n (replace_nth n v l) = firstn n l.
+Proof.
+  revert l v.
+  induction n; intros; destruct l; simpl; auto; f_equal; apply IHn.
+Qed.
+
+Lemma length_replace_nth {A} (n: nat) (v: A) (l: list A) :
+  length (replace_nth n v l) = length l.
+Proof.
+  revert v l.
+  induction n; intros v l.
+  - destruct l; simpl; auto.
+  - destruct l; simpl.
+    + reflexivity.
+    + f_equal. apply IHn.
+Qed.
+
+Lemma nth_replace_nth {A} (n: nat) (v d: A) (l: list A) :
+  (n < length l)%nat ->
+  nth n (replace_nth n v l) d = v.
+Proof.
+  revert l.
+  induction n; intros l Hlen; destruct l; simpl in *; try lia; auto.
+  apply IHn; lia.
+Qed.
+
+
+Lemma sublist_replace_prefix {A} (l: list A) (i: Z) (v: A) :
+  0 <= i ->
+  sublist 0 i (replace_Znth i v l) = sublist 0 i l.
+Proof.
+  intros.
+  unfold sublist, replace_Znth.
+  rewrite firstn_replace_nth_nat.
+  reflexivity.
+Qed.
+
+Lemma Zlength_replace_Znth {A} (l: list A) (i: Z) (v: A) :
+  Zlength (replace_Znth i v l) = Zlength l.
+Proof.
+  unfold replace_Znth.
+  rewrite !Zlength_correct, length_replace_nth.
+  reflexivity.
+Qed.
+
+Lemma Znth_replace_eq {A} (l: list A) (i: Z) (v d: A) :
+  0 <= i < Zlength l ->
+  Znth i (replace_Znth i v l) d = v.
+Proof.
+  intros [Hi0 Hi1].
+  unfold replace_Znth, Znth.
+  replace (Z.to_nat i) with (Z.to_nat i + 0)%nat by lia.
+  apply nth_replace_nth.
+  rewrite Zlength_correct in Hi1.
+  apply Z2Nat.inj_lt in Hi1; lia.
+Qed.
+
+Lemma zeros_succ : forall n, 0 <= n -> zeros (n + 1) = zeros n ++ (0 :: nil).
+Proof.
+  intros.
+  unfold zeros.
+  rewrite Z2Nat.inj_add by lia.
+  simpl.
+  rewrite repeat_app.
+  simpl.
+  reflexivity.
+Qed.
+
+Lemma store_map_empty :
+  forall {A B} (P: A -> B -> Assertion),
+    store_map P (@empty_map A B) --||-- emp.
+Proof.
+  intros A B P.
+  unfold store_map, empty_map.
+  unfold logic_equiv, derivable1.
+  unfold exp, andp, coq_prop, iter_sepcon, emp.
+  split.
+  - intros st H.
+    destruct H as [l [[HIn HNoDup] HIter]].
+    destruct l.
+    + exact HIter.
+    + exfalso.
+      match goal with
+      | HIn0: (forall x, In x (?hd :: ?tl) <-> exists b, None = Some b) |- _ =>
+          pose proof (HIn0 hd) as Hhd;
+          assert (In hd (hd :: tl)) as Hin by (simpl; auto);
+          apply Hhd in Hin;
+          destruct Hin as [b Hb];
+          discriminate Hb
+      end.
+  - intros st Hemp.
+    exists (@nil A).
+    split.
+    + split.
+      * intros a; split; intros Hin.
+        { inversion Hin. }
+        { destruct Hin as [b Hb]. discriminate Hb. }
+      * constructor.
+    + exact Hemp.
+Qed.
+
+Lemma dup_store_uint : forall p v1 v2,
+  p # UInt |-> v1 ** p # UInt |-> v2 |-- [| False |].
+Proof.
+  intros.
+  sep_apply store_uint_undef_store_uint.
+  sep_apply store_uint_undef_store_uint.
+  unfold undef_store_uint.
+  eapply derivable1_trans.
+  2: apply (dup_store_4bytes_noninit p).
+  entailer!.
+Qed.
+
+Lemma dup_store_val : forall p v1 v2,
+  store_val p v1 ** store_val p v2 |-- [| False |].
+Proof.
+  intros.
+  unfold store_val.
+  apply dup_store_uint.
+Qed.
+
+Lemma store_val_to_field : forall p v,
+  store_val p v |-- (&(p # "blist" ->ₛ "val")) # UInt |-> v.
+Proof.
+  intros.
+  unfold store_val.
+  entailer!.
+Qed.
+
+Lemma store_val_from_field : forall p v,
+  (&(p # "blist" ->ₛ "val")) # UInt |-> v |-- store_val p v.
+Proof.
+  intros.
+  unfold store_val.
+  entailer!.
+Qed.
+
+(* Axiom store_name_from_key :
+  forall p key_pre k,
+    &(p # "blist" ->ₛ "key") # Ptr |-> key_pre ** store_string key_pre k
+    |-- store_name k p. *)
+
+(* Axiom dll_singleton_from_fields :
+  forall x x_up x_down,
+    x <> NULL ->
+    &(x # "blist" ->ₛ "down") # Ptr |-> x_down **
+    &(x # "blist" ->ₛ "up") # Ptr |-> x_up
+    |-- dll x x_up (x :: nil). *)
+
+Lemma store_hash_skeleton_intro :
+  forall (x: addr) (m: list Z -> option addr)
+         (l lh: list addr) (b: Z -> option (addr * list addr))
+         (top bucks: addr),
+    (&(x # "hashtbl" ->ₛ "top") # Ptr |-> top **
+     &(x # "hashtbl" ->ₛ "bucks") # Ptr |-> bucks) **
+    PtrArray.full bucks 211 lh
+    |-- store_hash_skeleton x m.
+Proof.
+  pre_process.
+  unfold store_hash_skeleton.
+Abort.
+
+
+Definition hash_skeleton_inputs
+           (x: addr) (l lh: list addr) (b: Z -> option (addr * list addr))
+           (top bucks old_top old_down old_up next: addr)
+           (m: list Z -> option addr) : Assertion :=
+  (((((((( &(x # "hashtbl" ->ₛ "top") # Ptr |-> top **
+           dll top NULL l) **
+          &(x # "hashtbl" ->ₛ "bucks") # Ptr |-> bucks) **
+         PtrArray.full bucks 211 lh) **
+        store_map store_sll b) **
+       store_map store_name m) **
+      &(old_top # "blist" ->ₛ "down") # Ptr |-> old_down) **
+     &(old_top # "blist" ->ₛ "up") # Ptr |-> old_up) **
+    &(top # "blist" ->ₛ "next") # Ptr |-> next).
+
+
+Lemma dll_head_exists_with_TT :
+  forall x y l,
+    x <> NULL ->
+    dll x y l |-- EX x_down x_up l_tail,
+      [| l = x :: l_tail |] &&
+      &(x # "blist" ->ₛ "down") # Ptr |-> x_down **
+      &(x # "blist" ->ₛ "up") # Ptr |-> x_up **
+      TT.
+Proof.
+  intros x y l Hx.
+  sep_apply (dll_not_zero x y l Hx).
+  Intros x_down l_tail.
+  Exists x_down y l_tail.
+  entailer!.
+  apply derivable1_truep_intros.
+Qed.
+
+(* ---------------------------------------------------------------------- *)
+(* Proofs                                                                 *)
+(* ---------------------------------------------------------------------- *)
+
+Lemma proof_of_create_bucks_entail_wit_1 : create_bucks_entail_wit_1.
+Proof.
+  pre_process.
+  Exists content_2 retval.
+  rewrite sublist_nil by lia.
+  simpl.
+  entailer!.
+Qed.
+
+Lemma proof_of_create_bucks_entail_wit_2 : create_bucks_entail_wit_2.
+Proof.
+  pre_process.
+  rename H into Hi_lt.
+  rename H0 into Hi_nonneg.
+  rename H1 into Hi_le.
+  rename H2 into Hprefix.
+  rename H3 into Hretval.
+  Exists (replace_Znth i 0 content_2) bucks_base_2.
+  prop_apply PtrArray.full_Zlength; Intros.
+  match goal with
+  | H : Zlength (replace_Znth _ _ _) = _ |- _ =>
+      pose proof H as Hlen_repl
+  end.
+  pose proof Hlen_repl as Hlen_nat.
+  rewrite Zlength_correct in Hlen_nat.
+  assert (Hlen : Zlength content_2 = 211) by
+    (rewrite <- (Zlength_replace_Znth content_2 i 0); exact Hlen_repl).
+  assert (Hsplit: sublist 0 (i + 1) (replace_Znth i 0 content_2) =
+                  sublist 0 i (replace_Znth i 0 content_2) ++
+                  sublist i (i + 1) (replace_Znth i 0 content_2)) by
+    (apply sublist_split; [lia| rewrite Hlen_nat; lia]).
+  rewrite Hsplit.
+  rewrite (sublist_replace_prefix content_2 i 0) by lia.
+  rewrite (sublist_single i (replace_Znth i 0 content_2) 0) by (rewrite Hlen_nat; lia).
+  rewrite (Znth_replace_eq content_2 i 0 0) by (rewrite Hlen; lia).
+  rewrite Hprefix.
+  rewrite zeros_succ by lia.
+  entailer!.
+Qed.
+
+Lemma proof_of_create_bucks_return_wit_1 : create_bucks_return_wit_1.
+Proof.
+  pre_process.
+  rename H into Hi_ge.
+  rename H0 into Hi_nonneg.
+  rename H1 into Hi_le.
+  rename H2 into Hprefix.
+  rename H3 into Hretval.
+  assert (i = 211) by lia; subst i.
+  prop_apply (PtrArray.full_Zlength bucks_base_2 211 content); Intros.
+  match goal with
+  | H : Zlength content = _ |- _ => pose proof H as Hlen
+  end.
+  assert (content = zeros 211).
+  { assert (Hsub : sublist 0 211 content = content).
+    { apply sublist_self; rewrite Hlen; reflexivity. }
+    apply (eq_trans (eq_sym Hprefix)) in Hsub.
+    symmetry; exact Hsub. }
+  subst content.
+  Exists bucks_base_2.
+  entailer!.
+Qed.
+
+(* -------- init_hashtbl -------- *)
+
+
+
+
+Lemma proof_of_init_hashtbl_return_wit_1 : init_hashtbl_return_wit_1.
+Proof.
+  pre_process.
+  sep_apply (store_hash_skeleton_intro h_pre empty_map nil (zeros 211) empty_map 0 bucks_base).
+  entailer!.
+Qed.
+
+(* -------- create_hashtbl -------- *)
+
+Lemma proof_of_create_hashtbl_return_wit_1 : create_hashtbl_return_wit_1.
+Proof.
+  pre_process.
+  apply derivable1s_emp_sepcon_unfold.
+  - apply derivable1_refl.
+  - setoid_rewrite <- (store_map_empty store_val).
+    entailer!.
+Qed.
+
+(* -------- hashtbl_add -------- *)
+
+Lemma proof_of_hashtbl_add_entail_wit_1 : hashtbl_add_entail_wit_1.
+Proof.
+  pre_process.
+  entailer!.
+  - pose proof (Z.rem_bound_pos retval 211) as Hrem.
+    lia.
+  - pose proof (Z.rem_nonneg retval 211) as Hrem.
+    lia.
+Qed. 
+
+
+Lemma proof_of_hashtbl_add_return_wit_1 : hashtbl_add_return_wit_1.
+Proof.
+  pre_process.
+  Exists retval_2.
+  destruct (m2 retval_2) eqn:Hm2_at_new.
+  - match goal with
+    | H : m2 retval_2 = Some ?v |- _ => rename v into v_old
+    end.
+    sep_apply (store_map_split store_val retval_2 v_old m2 Hm2_at_new).
+    sep_apply store_val_to_field.
+    sep_apply (dup_store_uint (&(retval_2 # "blist" ->ₛ "val")) v_old val_pre).
+    entailer!.
+  - set (m2' := PV.insert_map m2 retval_2 val_pre).
+    sep_apply (store_map_equiv_store_map_missing store_val m2 retval_2 Hm2_at_new).
+    assert (Houtside : forall a, a <> retval_2 -> m2 a = m2' a).
+    { intros a Ha.
+      unfold m2'.
+      symmetry.
+      rewrite PV.insert_map_diff by congruence.
+      reflexivity. }
+    pose proof (store_map_missing_i_equiv store_val m2 m2' retval_2 Houtside) as Heq.
+    destruct Heq as [Hmiss _].
+    sep_apply Hmiss.
+    assert (Hm2'_at_new : m2' retval_2 = Some val_pre).
+    { unfold m2'. apply PV.insert_map_same. }
+    sep_apply store_val_from_field.
+    sep_apply (store_map_merge store_val retval_2 val_pre m2' Hm2'_at_new).
+    sep_apply (store_hash_skeleton_intro
+                 h_pre
+                 (KP.insert_map m1 k retval_2)
+                 l
+                 (replace_Znth (retval % 211) retval_2 lh)
+                 b
+                 retval_2
+                 bucks_ph).
+    unfold m2' in *.
+    unfold store_hash_skeleton.
+    Intros l0 lh0 b0 top0 bucks0.
+    assert (Hins_k : KP.insert_map m1 k retval_2 k = Some retval_2) by
+      apply KP.insert_map_same.
+    sep_apply (store_map_split store_name k retval_2 (KP.insert_map m1 k retval_2) Hins_k).
+    unfold store_name.
+    Intros key_ptr.
+    sep_apply (dup_store_ptr (&(retval_2 # "blist" ->ₛ "key")) key_ptr key_pre).
+    entailer!.
+Qed.
+      
+Lemma proof_of_hashtbl_add_return_wit_2 : hashtbl_add_return_wit_2.
+Proof.
+  pre_process.
+  Exists retval_2.
+  destruct (m2 retval_2) eqn:Hm2_at_new.
+  - match goal with
+    | H : m2 retval_2 = Some ?v |- _ => rename v into v_old
+    end.
+    sep_apply (store_map_split store_val retval_2 v_old m2 Hm2_at_new).
+    sep_apply store_val_to_field.
+    sep_apply (dup_store_uint (&(retval_2 # "blist" ->ₛ "val")) v_old val_pre).
+    entailer!.
+  - set (m2' := PV.insert_map m2 retval_2 val_pre).
+    sep_apply (store_map_equiv_store_map_missing store_val m2 retval_2 Hm2_at_new).
+    assert (Houtside : forall a, a <> retval_2 -> m2 a = m2' a).
+    { intros a Ha.
+      unfold m2'.
+      symmetry.
+      rewrite PV.insert_map_diff by congruence.
+      reflexivity. }
+    pose proof (store_map_missing_i_equiv store_val m2 m2' retval_2 Houtside) as Heq.
+    destruct Heq as [Hmiss _].
+    sep_apply Hmiss.
+    assert (Hm2'_at_new : m2' retval_2 = Some val_pre).
+    { unfold m2'. apply PV.insert_map_same. }
+    sep_apply store_val_from_field.
+    sep_apply (store_map_merge store_val retval_2 val_pre m2' Hm2'_at_new).
+    sep_apply (store_hash_skeleton_intro
+                 h_pre
+                 (KP.insert_map m1 k retval_2)
+                 (retval_2 :: l)
+                 (replace_Znth (retval % 211) retval_2 lh)
+                 b
+                 retval_2
+                 bucks_ph).
+    unfold m2' in *.
+    unfold store_hash_skeleton.
+    Intros l0 lh0 b0 top0 bucks0.
+    assert (Hins_k : KP.insert_map m1 k retval_2 k = Some retval_2) by
+      apply KP.insert_map_same.
+    sep_apply (store_map_split store_name k retval_2 (KP.insert_map m1 k retval_2) Hins_k).
+    unfold store_name.
+    Intros key_ptr.
+    sep_apply (dup_store_ptr (&(retval_2 # "blist" ->ₛ "key")) key_ptr key_pre).
+    entailer!.
+Qed.
+
+
+Lemma proof_of_hashtbl_add_which_implies_wit_1 : hashtbl_add_which_implies_wit_1.
+Proof. 
+  pre_process.
+  unfold store_hash_skeleton.
+  Intros l lh b top bucks.
+  unfold NBUCK, NULL.
+  Exists b lh l bucks top.
+  eapply sepcon_cancel_end.
+  - entailer!.
+  - apply derivable1_truep_intros.
+Qed.
+
+Lemma proof_of_hashtbl_add_which_implies_wit_2 : hashtbl_add_which_implies_wit_2.
+Proof.
+  pre_process.
+  assert (top_ph <> NULL) as Htop by (unfold NULL; auto).
+  sep_apply (dll_head_exists_with_TT top_ph 0 l Htop).
+  Intros top_down top_up l_tail.
+  Exists top_up top_down l_tail.
+  entailer!.
+Qed.
+ *)
+Require Import Coq.ZArith.ZArith.
+Require Import Coq.Bool.Bool.
+Require Import Coq.Strings.String.
+Require Import Coq.Lists.List.
+Require Import Coq.Classes.RelationClasses.
+Require Import Coq.Classes.Morphisms.
+Require Import Coq.micromega.Psatz.
+Require Import Coq.Sorting.Permutation.
+From AUXLib Require Import int_auto Axioms Feq Idents List_lemma VMap.
+Require Import SetsClass.SetsClass. Import SetsNotation.
+From SimpleC.SL Require Import Mem SeparationLogic MapLib CommonAssertion.
+Require Import Logic.SeparationLogic.ProofTheory.SeparationLogic.
+Require Import hashtbl_goal.
+Require Import Logic.LogicGenerator.demo932.Interface.
+Local Open Scope Z_scope.
+Local Open Scope sets.
+Local Open Scope string.
+Local Open Scope list.
+Import naive_C_Rules.
+Require Import hashtbl_lib.
+Local Open Scope sac.
+
+Module BV.
+  Definition insert_map {A} (m: Z -> option A) (k: Z) (v: A) : Z -> option A :=
+    fun x => if Z.eq_dec x k then Some v else m x.
+
+  Lemma insert_map_same {A} : forall (m: Z -> option A) k v,
+    insert_map m k v k = Some v.
+  Proof.
+    intros. unfold insert_map. destruct (Z.eq_dec k k); congruence.
+  Qed.
+
+  Lemma insert_map_diff {A} : forall (m: Z -> option A) k1 k2 v,
+    k1 <> k2 -> insert_map m k1 v k2 = m k2.
+  Proof.
+    intros. unfold insert_map. destruct (Z.eq_dec k2 k1); congruence.
+  Qed.
+
+  Lemma insert_map_iff {A} : forall (m: Z -> option A) k v p,
+    insert_map m k v p <> None <-> (p = k \/ m p <> None).
+  Proof.
+    intros. unfold insert_map. destruct (Z.eq_dec p k).
+    - subst. split; intros.
+      + left; auto.
+      + congruence.
+    - split; intros.
+      + right. auto.
+      + destruct H; try congruence.
+  Qed.
+End BV.
+
+
+
+
+
+(* ---------------------------------------------------------------------- *)
+(* Helper lemmas about lists                                               *)
+(* ---------------------------------------------------------------------- *)
+
+Lemma firstn_replace_nth_nat {A} (n: nat) (v: A) (l: list A) :
+  firstn n (replace_nth n v l) = firstn n l.
+Proof.
+  revert l v.
+  induction n; intros; destruct l; simpl; auto; f_equal; apply IHn.
+Qed.
+
+Lemma length_replace_nth {A} (n: nat) (v: A) (l: list A) :
+  length (replace_nth n v l) = length l.
+Proof.
+  revert v l.
+  induction n; intros v l.
+  - destruct l; simpl; auto.
+  - destruct l; simpl.
+    + reflexivity.
+    + f_equal. apply IHn.
+Qed.
+
+Lemma nth_replace_nth {A} (n: nat) (v d: A) (l: list A) :
+  (n < length l)%nat ->
+  nth n (replace_nth n v l) d = v.
+Proof.
+  revert l.
+  induction n; intros l Hlen; destruct l; simpl in *; try lia; auto.
+  apply IHn; lia.
+Qed.
+
+
+Lemma sublist_replace_prefix {A} (l: list A) (i: Z) (v: A) :
+  0 <= i ->
+  sublist 0 i (replace_Znth i v l) = sublist 0 i l.
+Proof.
+  intros.
+  unfold sublist, replace_Znth.
+  rewrite firstn_replace_nth_nat.
+  reflexivity.
+Qed.
+
+Lemma Zlength_replace_Znth {A} (l: list A) (i: Z) (v: A) :
+  Zlength (replace_Znth i v l) = Zlength l.
+Proof.
+  unfold replace_Znth.
+  rewrite !Zlength_correct, length_replace_nth.
+  reflexivity.
+Qed.
+
+Lemma Znth_replace_eq {A} (l: list A) (i: Z) (v d: A) :
+  0 <= i < Zlength l ->
+  Znth i (replace_Znth i v l) d = v.
+Proof.
+  intros [Hi0 Hi1].
+  unfold replace_Znth, Znth.
+  replace (Z.to_nat i) with (Z.to_nat i + 0)%nat by lia.
+  apply nth_replace_nth.
+  rewrite Zlength_correct in Hi1.
+  apply Z2Nat.inj_lt in Hi1; lia.
+Qed.
+
+Lemma zeros_succ : forall n, 0 <= n -> zeros (n + 1) = zeros n ++ (0 :: nil).
+Proof.
+  intros.
+  unfold zeros.
+  rewrite Z2Nat.inj_add by lia.
+  simpl.
+  rewrite repeat_app.
+  simpl.
+  reflexivity.
+Qed.
+
+Lemma store_map_empty :
+  forall {A B} (P: A -> B -> Assertion),
+    store_map P (@empty_map A B) --||-- emp.
+Proof.
+  intros A B P.
+  unfold store_map, empty_map.
+  unfold logic_equiv, derivable1.
+  unfold exp, andp, coq_prop, iter_sepcon, emp.
+  split.
+  - intros st H.
+    destruct H as [l [[HIn HNoDup] HIter]].
+    destruct l.
+    + exact HIter.
+    + exfalso.
+      match goal with
+      | HIn0: (forall x, In x (?hd :: ?tl) <-> exists b, None = Some b) |- _ =>
+          pose proof (HIn0 hd) as Hhd;
+          assert (In hd (hd :: tl)) as Hin by (simpl; auto);
+          apply Hhd in Hin;
+          destruct Hin as [b Hb];
+          discriminate Hb
+      end.
+  - intros st Hemp.
+    exists (@nil A).
+    split.
+    + split.
+      * intros a; split; intros Hin.
+        { inversion Hin. }
+        { destruct Hin as [b Hb]. discriminate Hb. }
+      * constructor.
+    + exact Hemp.
+Qed.
+
+Lemma dup_store_uint : forall p v1 v2,
+  p # UInt |-> v1 ** p # UInt |-> v2 |-- [| False |].
+Proof.
+  intros.
+  sep_apply store_uint_undef_store_uint.
+  sep_apply store_uint_undef_store_uint.
+  unfold undef_store_uint.
+  eapply derivable1_trans.
+  2: apply (dup_store_4bytes_noninit p).
+  entailer!.
+Qed.
+
+Lemma dup_store_val : forall p v1 v2,
+  store_val p v1 ** store_val p v2 |-- [| False |].
+Proof.
+  intros.
+  unfold store_val.
+  apply dup_store_uint.
+Qed.
+
+Lemma store_val_to_field : forall p v,
+  store_val p v |-- (&(p # "blist" ->ₛ "val")) # UInt |-> v.
+Proof.
+  intros.
+  unfold store_val.
+  entailer!.
+Qed.
+
+Lemma store_val_from_field : forall p v,
+  (&(p # "blist" ->ₛ "val")) # UInt |-> v |-- store_val p v.
+Proof.
+  intros.
+  unfold store_val.
+  entailer!.
+Qed.
+
+Lemma store_name_intro : forall p key_ptr k,
+  (&(p # "blist" ->ₛ "key")) # Ptr |-> key_ptr ** store_string key_ptr k
+  |-- store_name k p.
+Proof.
+  intros.
+  unfold store_name.
+  Exists key_ptr.
+  entailer!.
+Qed.
+
+(* Axiom store_name_from_key :
+  forall p key_pre k,
+    &(p # "blist" ->ₛ "key") # Ptr |-> key_pre ** store_string key_pre k
+    |-- store_name k p. *)
+
+(* Axiom dll_singleton_from_fields :
+  forall x x_up x_down,
+    x <> NULL ->
+    &(x # "blist" ->ₛ "down") # Ptr |-> x_down **
+    &(x # "blist" ->ₛ "up") # Ptr |-> x_up
+    |-- dll x x_up (x :: nil). *)
+
+Lemma store_hash_skeleton_intro :
+  forall (x: addr) (m: list Z -> option addr)
+         (l lh: list addr) (b: Z -> option (addr * list addr))
+         (top bucks: addr),
+    (&(x # "hashtbl" ->ₛ "top") # Ptr |-> top ** dll top NULL l) **
+    (&(x # "hashtbl" ->ₛ "bucks") # Ptr |-> bucks ** PtrArray.full bucks 211 lh) **
+    store_map store_sll b ** store_map store_name m
+    |-- store_hash_skeleton x m.
+Proof.
+  pre_process.
+  unfold store_hash_skeleton.
+  Exists l lh b top bucks.
+  entailer!.
+Qed.
+
+
+Definition hash_skeleton_inputs
+           (x: addr) (l lh: list addr) (b: Z -> option (addr * list addr))
+           (top bucks old_top old_down old_up next: addr)
+           (m: list Z -> option addr) : Assertion :=
+  (((((((( &(x # "hashtbl" ->ₛ "top") # Ptr |-> top **
+           dll top NULL l) **
+          &(x # "hashtbl" ->ₛ "bucks") # Ptr |-> bucks) **
+         PtrArray.full bucks 211 lh) **
+        store_map store_sll b) **
+       store_map store_name m) **
+      &(old_top # "blist" ->ₛ "down") # Ptr |-> old_down) **
+     &(old_top # "blist" ->ₛ "up") # Ptr |-> old_up) **
+    &(top # "blist" ->ₛ "next") # Ptr |-> next).
+
+
+Lemma dll_head_exists_with_TT :
+  forall x y l,
+    x <> NULL ->
+    dll x y l |-- EX x_down x_up l_tail,
+      [| l = x :: l_tail |] &&
+      &(x # "blist" ->ₛ "down") # Ptr |-> x_down **
+      &(x # "blist" ->ₛ "up") # Ptr |-> x_up **
+      TT.
+Proof.
+  intros x y l Hx.
+  sep_apply (dll_not_zero x y l Hx).
+  Intros x_down l_tail.
+  Exists x_down y l_tail.
+  entailer!.
+  apply derivable1_truep_intros.
+Qed.
+
+(* ---------------------------------------------------------------------- *)
+(* Proofs                                                                 *)
+(* ---------------------------------------------------------------------- *)
+
+Lemma proof_of_create_bucks_entail_wit_1 : create_bucks_entail_wit_1.
+Proof.
+  pre_process.
+  Exists content_2 retval.
+  rewrite sublist_nil by lia.
+  simpl.
+  entailer!.
+Qed.
+
+Lemma proof_of_create_bucks_entail_wit_2 : create_bucks_entail_wit_2.
+Proof.
+  pre_process.
+  rename H into Hi_lt.
+  rename H0 into Hi_nonneg.
+  rename H1 into Hi_le.
+  rename H2 into Hprefix.
+  rename H3 into Hretval.
+  Exists (replace_Znth i 0 content_2) bucks_base_2.
+  prop_apply PtrArray.full_Zlength; Intros.
+  match goal with
+  | H : Zlength (replace_Znth _ _ _) = _ |- _ =>
+      pose proof H as Hlen_repl
+  end.
+  pose proof Hlen_repl as Hlen_nat.
+  rewrite Zlength_correct in Hlen_nat.
+  assert (Hlen : Zlength content_2 = 211) by
+    (rewrite <- (Zlength_replace_Znth content_2 i 0); exact Hlen_repl).
+  assert (Hsplit: sublist 0 (i + 1) (replace_Znth i 0 content_2) =
+                  sublist 0 i (replace_Znth i 0 content_2) ++
+                  sublist i (i + 1) (replace_Znth i 0 content_2)) by
+    (apply sublist_split; [lia| rewrite Hlen_nat; lia]).
+  rewrite Hsplit.
+  rewrite (sublist_replace_prefix content_2 i 0) by lia.
+  rewrite (sublist_single i (replace_Znth i 0 content_2) 0) by (rewrite Hlen_nat; lia).
+  rewrite (Znth_replace_eq content_2 i 0 0) by (rewrite Hlen; lia).
+  rewrite Hprefix.
+  rewrite zeros_succ by lia.
+  entailer!.
+Qed.
+
+Lemma proof_of_create_bucks_return_wit_1 : create_bucks_return_wit_1.
+Proof.
+  pre_process.
+  rename H into Hi_ge.
+  rename H0 into Hi_nonneg.
+  rename H1 into Hi_le.
+  rename H2 into Hprefix.
+  rename H3 into Hretval.
+  assert (i = 211) by lia; subst i.
+  prop_apply (PtrArray.full_Zlength bucks_base_2 211 content); Intros.
+  match goal with
+  | H : Zlength content = _ |- _ => pose proof H as Hlen
+  end.
+  assert (content = zeros 211).
+  { assert (Hsub : sublist 0 211 content = content).
+    { apply sublist_self; rewrite Hlen; reflexivity. }
+    apply (eq_trans (eq_sym Hprefix)) in Hsub.
+    symmetry; exact Hsub. }
+  subst content.
+  Exists bucks_base_2.
+  entailer!.
+Qed.
+
+(* -------- init_hashtbl -------- *)
+
+
+
+
+Lemma proof_of_init_hashtbl_return_wit_1 : init_hashtbl_return_wit_1.
+Proof.
+  pre_process.
+  unfold store_hash_skeleton.
+  Exists nil (zeros 211) empty_map 0 bucks_base.
+  setoid_rewrite (store_map_empty store_sll).
+  setoid_rewrite (store_map_empty store_name).
+  simpl dll.
+  unfold NULL.
+  entailer!.
+Qed.
+
+(* -------- create_hashtbl -------- *)
+
+Lemma proof_of_create_hashtbl_return_wit_1 : create_hashtbl_return_wit_1.
+Proof.
+  pre_process.
+  apply derivable1s_emp_sepcon_unfold.
+  - apply derivable1_refl.
+  - setoid_rewrite <- (store_map_empty store_val).
+    entailer!.
+Qed.
